wrote demands_analysis_fun

meta-theory/pure_demandScript.sml
@@ -1,6 +1,7 @@
 (*
    Formalises the notion of "demand" as used in demand/strictness analysis.
 *)
+
 open HolKernel Parse boolLib bossLib term_tactic;
 open arithmeticTheory listTheory stringTheory alistTheory dep_rewrite
      optionTheory pairTheory ltreeTheory llistTheory bagTheory
@@ -15,56 +16,157 @@ Definition Projs_def:
   Projs ((x,i)::ps) e = Projs ps (Proj x i e)
 End
 
-val _ = set_fixity "demands" (Infixl 480);
+Theorem demands_proj_end:
+  ∀ ps x i e. Projs (ps++[(x,i)]) e = Proj x i (Projs ps e)
+Proof
+  Induct THEN1 rw [Projs_def]
+  \\ gen_tac \\ rename1 ‘hd::ps’
+  \\ PairCases_on ‘hd’
+  \\ rw [Projs_def]
+QED
 
-Definition demands_def:
-  (e demands (p,v)) = (e ≅ Seq (Projs p (Var v)) e)
+Theorem double_Projs:
+  ∀ps' ps e. Projs (ps' ++ ps) e = Projs ps (Projs ps' e)
+Proof
+  Induct >- rw [Projs_def]
+  \\ gen_tac \\ rename1 ‘hd::ps'’
+  \\ PairCases_on ‘hd’
+  \\ rw [Projs_def]
+QED
+
+Theorem Seq_App:
+  ∀b. (App (Seq p f) e ≅? Seq p (App f e)) b
+Proof
+  irule eval_wh_IMP_exp_eq
+  \\ rw [subst_def, eval_wh_App, eval_wh_Seq]
+  \\ fs []
+QED
+
+Theorem Proj_Seq2:
+  ∀b. (Proj x i (Seq e e') ≅? Seq e (Proj x i e')) b
+Proof
+  irule eval_wh_IMP_exp_eq
+  \\ rw [subst_def, eval_wh_Proj, eval_wh_Seq]
+  \\ fs []
+QED
+
+Theorem If_Seq:
+  ∀e e' e'' e''' b. (If (Seq e e') e'' e''' ≅? Seq e (If e' e'' e''')) b
+Proof
+  rpt gen_tac
+  \\ irule eval_wh_IMP_exp_eq
+  \\ rw [subst_def, eval_wh_If, eval_wh_Seq]
+  \\ fs []
+QED
+
+Theorem Seq_comm:
+  Seq (Seq x y) z ≈ Seq (Seq y x) z
+Proof
+  irule no_err_eval_wh_IMP_exp_eq
+  \\ rw [subst_def, no_err_eval_wh_def, eval_wh_Seq]
+  \\ fs []
+  \\ Cases_on ‘eval_wh (subst f x)’
+  \\ Cases_on ‘eval_wh (subst f y)’
+  \\ fs []
+QED
+
+Theorem If_Seq2:
+  ∀e ec et ee.  If ec (Seq e et) (Seq e ee) ≈ Seq e (If ec et ee)
+Proof
+  rpt gen_tac
+  \\ irule no_err_eval_wh_IMP_exp_eq
+  \\ rw [no_err_eval_wh_def, freevars_def, subst_def, eval_wh_If, eval_wh_Seq]
+  \\ fs []
+QED
+
+Theorem IsEq_Seq:
+  ∀b e e' n i. (IsEq n i (Seq e e') ≅? Seq e (IsEq n i e')) b
+Proof
+  rpt gen_tac
+  \\ irule eval_wh_IMP_exp_eq
+  \\ rw [subst_def, eval_wh_IsEq, eval_wh_Seq]
+  \\ fs []
+QED
+
+
+Definition well_written_def:
+  well_written (Cons s) l = T ∧
+  well_written (Proj s i) [e] = T ∧
+  well_written (IsEq s i) [e] = T ∧
+  well_written If [e; e'; e''] = T ∧
+  well_written Seq [e; e'] = T ∧
+  well_written (AtomOp op) l = T ∧
+  well_written _ _ = F
 End
 
-Theorem demands_Var:
-  (Var v) demands ([],v)
+Theorem not_well_written_is_fail:
+  ∀b ope l.
+    ¬ well_written ope l ⇒
+    (Prim ope l ≅? Fail) b
 Proof
-  fs [demands_def,Projs_def]
-  \\ metis_tac [Seq_id,exp_eq_sym]
+  rw []
+  \\ Cases_on ‘ope’
+  \\ fs [well_written_def]
+  \\ Cases_on ‘l’
+  >>~[‘Prim _ [] ≅? Fail’]
+  >- (fs [exp_eq_refl])
+  >- (irule eval_wh_IMP_exp_eq
+     \\ fs [subst_def, eval_wh_def, eval_wh_to_def])
+  >- (irule eval_wh_IMP_exp_eq
+     \\ fs [subst_def, eval_wh_def, eval_wh_to_def])
+  >- (irule eval_wh_IMP_exp_eq
+     \\ fs [subst_def, eval_wh_def, eval_wh_to_def])
+  \\ rename1 ‘hd::tl’
+  \\ Cases_on ‘tl’
+  \\ fs [well_written_def]
+  >>~[‘Prim _ [hd]’]
+  >- (irule eval_wh_IMP_exp_eq
+     \\ fs [subst_def, eval_wh_def, eval_wh_to_def])
+  >- (irule eval_wh_IMP_exp_eq
+     \\ fs [subst_def, eval_wh_def, eval_wh_to_def])
+  \\ rename1 ‘h0::h1::tl’
+  \\ Cases_on ‘tl’
+  \\ fs [well_written_def]
+  >~[‘Prim If (h0::h1::h2::tl)’]
+  >- (Cases_on ‘tl’
+      \\ fs [well_written_def]
+      \\ irule eval_wh_IMP_exp_eq
+      \\ fs [subst_def, eval_wh_def, eval_wh_to_def])
+  \\ irule eval_wh_IMP_exp_eq
+  \\ fs [subst_def, eval_wh_def, eval_wh_to_def]
 QED
 
-Theorem demands_Proj:
-  e demands (ps,v) ⇒
-  (Proj n i e) demands (ps,v)
+Theorem exp_eq_l_refl:
+  ∀b l. LIST_REL (λx y. (x ≅? y) b) l l
 Proof
-  rw [demands_def,Projs_def]
-  \\ irule exp_eq_trans
-  \\ qexists_tac ‘Seq e (Proj n i e)’
-  \\ conj_tac THEN1 fs [Proj_Seq]
-  \\ qabbrev_tac ‘p = Projs ps (Var v)’
-  \\ irule exp_eq_trans
-  \\ qexists_tac ‘Seq (Seq p e) (Proj n i e)’
-  \\ conj_tac THEN1
-   (irule exp_eq_Prim_cong \\ fs [exp_eq_refl])
-  \\ irule exp_eq_trans
-  \\ qexists_tac ‘Seq p (Seq e (Proj n i e))’
-  \\ conj_tac THEN1 fs [Seq_assoc]
-  \\ irule exp_eq_Prim_cong \\ fs [exp_eq_refl,Let_Var]
-  \\ metis_tac [Proj_Seq,exp_eq_sym]
-QED
-
-Theorem demands_Proj_Var:
-  (Proj s i (Var v)) demands ([(s,i)],v)
-Proof
-  rw [demands_def,Projs_def]
-  \\ metis_tac [Seq_id,exp_eq_sym]
+  gen_tac
+  \\ Induct
+  \\ fs [exp_eq_refl]
 QED
 
 Theorem exp_eq_Projs_cong:
-  ∀ps x y. x ≅ y ⇒ Projs ps x ≅ Projs ps y
+  ∀ps x y b. (x ≅? y) b ⇒ (Projs ps x ≅? Projs ps y) b
 Proof
   Induct \\ fs [Projs_def,FORALL_PROD]
   \\ rw [] \\ first_x_assum irule
   \\ irule exp_eq_Prim_cong \\ fs [exp_eq_refl,Let_Var]
 QED
 
+Theorem Projs_Seq:
+  ∀ps e e' b. (Projs ps (Seq e e') ≅? Seq e (Projs ps e')) b
+Proof
+  Induct
+  THEN1 (rw [Projs_def] \\ fs [exp_eq_refl])
+  \\ rpt gen_tac
+  \\ rename1 ‘hd::ps’
+  \\ PairCases_on ‘hd’
+  \\ rw [Projs_def]
+  \\ irule exp_eq_trans \\ qexists_tac ‘Projs ps (Seq e (Proj hd0 hd1 e'))’
+  \\ fs [Proj_Seq2, exp_eq_sym, exp_eq_Projs_cong, Seq_id]
+QED
+
 Theorem Let_Projs:
-  ∀ps x w y. Let w y (Projs ps x) ≅ Projs ps (Let w y x)
+  ∀ps x w y b. (Let w y (Projs ps x) ≅? Projs ps (Let w y x)) b
 Proof
   Induct \\ fs [Projs_def,exp_eq_refl,FORALL_PROD] \\ rw []
   \\ irule exp_eq_trans
@@ -74,13 +176,139 @@ Proof
   \\ fs [Let_Prim_alt]
 QED
 
-Theorem demands_Let1:
-  e demands d ∧ e' demands ([],w) ⇒ (Let w e e') demands d
+Theorem Projs_subst:
+  ∀ps f e. subst f (Projs ps e) = Projs ps (subst f e)
+Proof
+  Induct THEN1 rw [Projs_def]
+  \\ gen_tac
+  \\ rename1 ‘Projs (hd::_) _’
+  \\ PairCases_on ‘hd’
+  \\ rw [Projs_def, subst_def]
+QED
+
+val _ = set_fixity "demands" (Infixl 480);
+
+Definition demands_def:
+  (e demands (p,v)) = (e ≈ Seq (Projs p (Var v)) e)
+End
+
+val _ = set_fixity "needs" (Infixl 480);
+Definition needs_def:
+  (e needs (ps, e')) = (e ≈ Seq (Projs ps e') e)
+End
+
+Theorem needs_Var_is_demands:
+  e needs (ps, Var v) ⇔ e demands (ps, v)
+Proof
+  rw [needs_def, demands_def] \\ fs []
+QED
+
+Theorem needs_refl:
+  ∀e. e needs ([],e)
+Proof
+  rw [needs_def, Projs_def]
+  \\ metis_tac [Seq_id, exp_eq_sym]
+QED
+
+Theorem needs_Var:
+  (Var v) needs ([], Var v)
+Proof
+  fs [needs_refl]
+QED
+
+Theorem needs_Proj:
+  e needs d ⇒ (Proj n i e) needs d
 Proof
   PairCases_on ‘d’
-  \\ rw [demands_def,Projs_def]
+  \\ rename1 ‘(ps, e')’
+  \\ rw [needs_def, Projs_def]
   \\ irule exp_eq_trans
-  \\ qabbrev_tac ‘p = (Projs d0 (Var d1))’
+  \\ qexists_tac ‘Seq e (Proj n i e)’
+  \\ conj_tac >- fs [Proj_Seq]
+  \\ qabbrev_tac ‘p = Projs ps e'’
+  \\ irule exp_eq_trans
+  \\ qexists_tac ‘Seq (Seq p e) (Proj n i e)’
+  \\ conj_tac
+  >- (irule exp_eq_Prim_cong \\ fs [exp_eq_refl])
+  \\ irule exp_eq_trans
+  \\ qexists_tac ‘Seq p (Seq e (Proj n i e))’
+  \\ conj_tac >- fs [Seq_assoc]
+  \\ irule exp_eq_Prim_cong \\ fs [exp_eq_refl, Let_Var]
+  \\ metis_tac [Proj_Seq, exp_eq_sym]
+QED
+
+Theorem needs_Projs:
+  ∀ps e d. e needs d ⇒ (Projs ps e) needs d
+Proof
+  Induct
+  >- rw [Projs_def]
+  \\ gen_tac \\ rename1 ‘(hd::ps)’ \\ PairCases_on ‘hd’
+  \\ rw [Projs_def]
+  \\ first_assum $ irule_at Any
+  \\ irule needs_Proj
+  \\ fs []
+QED
+
+Theorem needs_trans:
+  e needs (ps,e') ∧ e' needs (ps',e'') ⇒ e needs (ps',e'')
+Proof
+  rw [needs_def]
+  \\ irule exp_eq_trans
+  \\ first_assum $ irule_at Any
+  \\ irule exp_eq_trans
+  \\ qexists_tac ‘Seq (Seq (Projs ps' e'') (Projs ps e')) e’
+  \\ conj_tac >-
+   (irule exp_eq_Prim_cong \\ fs [exp_eq_refl]
+    \\ assume_tac needs_Projs \\ metis_tac [needs_def])
+  \\ irule exp_eq_trans
+  \\ qexists_tac ‘Seq (Projs ps' e'') (Seq (Projs ps e') e)’
+  \\ conj_tac >- fs [Seq_assoc]
+  \\ irule exp_eq_Prim_cong
+  \\ fs [exp_eq_refl, exp_eq_sym]
+QED
+
+Theorem needs_Projs_Var:
+  (Proj s i (Var v)) needs ([(s,i)], Var v)
+Proof
+  rw [needs_def, Projs_def]
+  \\ metis_tac [Seq_id, exp_eq_sym]
+QED
+
+Theorem needs_Seq:
+  e needs d ⇒ (Seq e e') needs d
+Proof
+  PairCases_on ‘d’
+  \\ rw [needs_def]
+  \\ irule exp_eq_trans
+  \\ qexists_tac ‘Seq (Seq (Projs d0 d1) e) e'’
+  \\ conj_tac >-
+   (irule exp_eq_Prim_cong \\ fs [exp_eq_refl])
+  \\ fs [Seq_assoc]
+QED
+
+
+Theorem needs_Seq2:
+  e' needs d ⇒ (Seq e e') needs d
+Proof
+  PairCases_on ‘d’
+  \\ rw [needs_def]
+  \\ irule exp_eq_trans
+  \\ qexists_tac ‘Seq e (Seq (Projs d0 d1) e')’
+  \\ fs [exp_eq_Prim_cong, exp_eq_refl]
+  \\ irule exp_eq_trans
+  \\ irule_at Any Seq_assoc
+  \\ irule exp_eq_trans
+  \\ irule_at Any Seq_comm
+  \\ metis_tac [Seq_assoc, exp_eq_sym]
+QED
+
+Theorem needs_Let1:
+  e needs d ∧ e' demands ([],w) ⇒ (Let w e e') needs d
+Proof
+  PairCases_on ‘d’
+  \\ rw [demands_def,needs_def,Projs_def]
+  \\ irule exp_eq_trans
+  \\ qabbrev_tac ‘p = (Projs d0 d1)’
   \\ qexists_tac ‘Let w e (Seq (Var w) e')’
   \\ conj_tac THEN1
    (irule exp_eq_App_cong \\ fs [exp_eq_refl]
@@ -102,18 +330,150 @@ Proof
   \\ irule exp_eq_Prim_cong \\ fs [exp_eq_refl]
   \\ once_rewrite_tac [exp_eq_sym]
   \\ irule exp_eq_trans
-  \\ qexists_tac ‘Let w e (Seq (Var w) e')’
+  \\ irule_at Any exp_eq_App_cong
+  \\ irule_at Any exp_eq_Lam_cong
+  \\ irule_at (Pos $ el 2) exp_eq_refl
+  \\ first_x_assum $ irule_at Any
+  \\ irule exp_eq_trans
+  \\ irule_at Any Let_Seq
+  \\ irule exp_eq_Prim_cong
+  \\ fs [exp_eq_refl, Let_Var]
+QED
+
+Theorem needs_Let_Cons: (* expects program to be in ANF *)
+  e demands ((s,LENGTH xs)::ps,w) ⇒
+  (Let w (Cons s (xs ++ e'::ys)) e) needs (ps,e')
+Proof
+  rw [demands_def,needs_def,Projs_def]
+  \\ qabbrev_tac ‘cons = (Cons s (xs ++ e'::ys))’
+  \\ irule exp_eq_trans
+  \\ qexists_tac ‘Let w cons (Seq (Projs ps (Proj s (LENGTH xs) (Var w))) e)’
   \\ conj_tac THEN1
    (irule exp_eq_App_cong \\ fs [exp_eq_refl]
     \\ irule exp_eq_Lam_cong \\ fs [exp_eq_refl])
   \\ irule exp_eq_trans
-  \\ qexists_tac ‘Seq (Let w e (Var w)) (Let w e e')’
-  \\ conj_tac THEN1 fs [Let_Seq]
+  \\ irule_at Any Let_Seq
+  \\ irule exp_eq_Prim_cong \\ fs [exp_eq_refl,Let_Var]
+  \\ fs [GSYM Projs_def]
   \\ irule exp_eq_trans
-  \\ qexists_tac ‘Seq e (Let w e e')’
+  \\ irule_at Any Let_Projs
+  \\ fs [Projs_def]
+  \\ irule exp_eq_Projs_cong \\ fs [exp_eq_refl,Let_Var]
+  \\ irule exp_eq_trans
+  \\ irule_at Any exp_eq_Prim_cong \\ fs [PULL_EXISTS]
+  \\ irule_at Any Let_Var
+  \\ unabbrev_all_tac
+  \\ fs [Proj_Cons]
+QED
+
+Theorem needs_Let_Proj: (* expects program to be in ANF *)
+  e demands (ps,w) ⇒
+  (Let w (Proj s i e') e) needs ((s,i)::ps,e')
+Proof
+  rw [demands_def,needs_def,Projs_def]
+  \\ irule exp_eq_trans
+  \\ qexists_tac ‘Let w (Proj s i e') (Seq (Projs ps (Var w)) e)’
   \\ conj_tac THEN1
-    (irule exp_eq_Prim_cong \\ fs [exp_eq_refl,Let_Var])
-  \\ fs [exp_eq_refl]
+   (irule exp_eq_App_cong \\ fs [exp_eq_refl]
+    \\ irule exp_eq_Lam_cong \\ fs [exp_eq_refl])
+  \\ irule exp_eq_trans
+  \\ qexists_tac ‘Seq (Let w (Proj s i e') (Projs ps (Var w)))
+                      (Let w (Proj s i e') e)’
+  \\ conj_tac THEN1 fs [Let_Seq]
+  \\ irule exp_eq_Prim_cong \\ fs [exp_eq_refl,Let_Var]
+  \\ irule exp_eq_trans
+  \\ qexists_tac ‘Projs ps (Let w (Proj s i e') (Var w))’
+  \\ conj_tac THEN1 fs [Let_Projs]
+  \\ irule exp_eq_Projs_cong
+  \\ fs [Let_Var]
+QED
+
+Theorem needs_App:
+  f needs d ⇒ (App f e) needs d
+Proof
+  PairCases_on ‘d’ \\ rename1 ‘(ps,e')’
+  \\ rw [needs_def]
+  \\ qabbrev_tac ‘proj = Projs ps e'’
+  \\ irule exp_eq_trans
+  \\ qexists_tac ‘App (Seq proj f) e’
+  \\ conj_tac THEN1
+   (irule exp_eq_App_cong \\ rw [exp_eq_refl])
+  \\ fs [Seq_App]
+QED
+
+Theorem needs_If:
+  e needs d ⇒ (If e e' e'') needs d
+Proof
+  PairCases_on ‘d’
+  \\ rw [needs_def]
+  \\ qabbrev_tac ‘p = Projs d0 d1’
+  \\ irule exp_eq_trans
+  \\ irule_at Any If_Seq
+  \\ irule exp_eq_Prim_cong
+  \\ fs [exp_eq_refl, exp_eq_sym]
+QED
+
+Theorem needs_If2:
+  et needs d ∧ ee needs d ⇒ (If ec et ee) needs d
+Proof
+  PairCases_on ‘d’
+  \\ rw [needs_def]
+  \\ irule exp_eq_trans
+  \\ irule_at Any If_Seq2
+  \\ irule exp_eq_Prim_cong
+  \\ fs [exp_eq_refl, exp_eq_sym]
+QED
+
+        (********************************************)
+
+Theorem demands_Var:
+  (Var v) demands ([],v)
+Proof
+  metis_tac [needs_Var_is_demands, needs_Var]
+QED
+
+Theorem demands_Proj:
+  e demands d ⇒
+  (Proj n i e) demands d
+Proof
+  PairCases_on ‘d’
+  \\ metis_tac [needs_Var_is_demands, needs_Proj]
+QED
+
+Theorem demands_Projs:
+  e demands d ⇒
+  (Projs ps2 e) demands d
+Proof
+  PairCases_on ‘d’
+  \\ metis_tac [needs_Var_is_demands, needs_Projs]
+QED
+
+Theorem demands_Proj_Var:
+  (Proj s i (Var v)) demands ([(s,i)],v)
+Proof
+  rw [demands_def,Projs_def]
+  \\ metis_tac [Seq_id,exp_eq_sym]
+QED
+
+Theorem demands_Seq:
+  e demands d ⇒ (Seq e e') demands d
+Proof
+  PairCases_on ‘d’
+  \\ metis_tac [needs_Var_is_demands, needs_Seq]
+QED
+
+Theorem demands_Seq2:
+  e' demands d ⇒ (Seq e e') demands d
+Proof
+  PairCases_on ‘d’
+  \\ metis_tac [needs_Var_is_demands, needs_Seq2]
+QED
+
+Theorem demands_Let1:
+  e demands d ∧ e' demands ([],w) ⇒ (Let w e e') demands d
+Proof
+  PairCases_on ‘d’
+  \\ metis_tac [needs_def, needs_Var_is_demands, needs_Let1]
 QED
 
 Theorem demands_Let2:
@@ -144,69 +504,1130 @@ Theorem demands_Let_Proj: (* expects program to be in ANF *)
   e demands (ps,w) ⇒
   (Let w (Proj s i (Var v)) e) demands ((s,i)::ps,v)
 Proof
-  rw [demands_def,Projs_def]
-  \\ irule exp_eq_trans
-  \\ qexists_tac ‘Let w (Proj s i (Var v)) (Seq (Projs ps (Var w)) e)’
-  \\ conj_tac THEN1
-   (irule exp_eq_App_cong \\ fs [exp_eq_refl]
-    \\ irule exp_eq_Lam_cong \\ fs [exp_eq_refl])
-  \\ irule exp_eq_trans
-  \\ qexists_tac ‘Seq (Let w (Proj s i (Var v)) (Projs ps (Var w)))
-                      (Let w (Proj s i (Var v)) e)’
-  \\ conj_tac THEN1 fs [Let_Seq]
-  \\ irule exp_eq_Prim_cong \\ fs [exp_eq_refl,Let_Var]
-  \\ irule exp_eq_trans
-  \\ qexists_tac ‘Projs ps (Let w (Proj s i (Var v)) (Var w))’
-  \\ conj_tac THEN1 fs [Let_Projs]
-  \\ irule exp_eq_Projs_cong
-  \\ fs [Let_Var]
+  metis_tac [needs_Let_Proj, needs_Var_is_demands]
 QED
 
 Theorem demands_Let_Cons: (* expects program to be in ANF *)
   e demands ((s,LENGTH xs)::ps,w) ⇒
   (Let w (Cons s (xs ++ (Var v)::ys)) e) demands (ps,v)
 Proof
-  rw [demands_def,Projs_def]
-  \\ qabbrev_tac ‘cons = (Cons s (xs ++ Var v::ys))’
+  metis_tac [needs_Let_Cons, needs_Var_is_demands]
+QED
+
+Theorem demands_App:
+  f demands d ⇒ (App f e) demands d
+Proof
+  PairCases_on ‘d’
+  \\ metis_tac [needs_App, needs_Var_is_demands]
+QED
+
+Theorem demands_If:
+  e demands d ⇒ (If e e' e'') demands d
+Proof
+  PairCases_on ‘d’
+  \\ metis_tac [needs_If, needs_Var_is_demands]
+QED
+
+Theorem demands_If2:
+  et demands d ∧ ee demands d ⇒ (If ec et ee) demands d
+Proof
+  PairCases_on ‘d’
+  \\ metis_tac [needs_If2, needs_Var_is_demands]
+QED
+
+Definition well_formed_def:
+  well_formed (Cons s) l = (s ≠ s) ∧
+  well_formed (Proj s i) l = (∃ e. l = [e]) ∧
+  well_formed (IsEq s i) l = (∃e. l = [e]) ∧
+  well_formed If (l: exp list) = (∃e e' e''. l = e::e'::e''::[]) ∧
+  well_formed Seq l = (∃e e'. l = e::e'::[]) ∧
+  well_formed (AtomOp op) l = (op ≠ op)
+End
+
+Theorem demands_Prim:
+  e demands d ∧ well_formed ope (e::l) ⇒ Prim ope (e::l) demands d
+Proof
+  PairCases_on ‘d’
+  \\ rw [demands_def]
+  \\ qabbrev_tac ‘p = Projs d0 (Var d1)’
+  \\ irule exp_eq_trans \\ qexists_tac ‘Prim ope ((Seq p e)::l)’
+  \\ conj_tac
+  >- (irule exp_eq_Prim_cong \\ fs [exp_eq_l_refl])
+  \\ Cases_on ‘ope’ \\ fs [well_formed_def]
+  \\ fs [If_Seq, IsEq_Seq, Proj_Seq2, Seq_assoc]
+QED
+
+Theorem demands_IsEq:
+  e demands d ⇒ (IsEq n i e) demands d
+Proof
+  strip_tac
+  \\ irule demands_Prim
+  \\ fs [well_formed_def]
+QED
+
+(*
+Definition is_good_def:
+  is_good e = (eval_wh e ≠ wh_Error ∧ eval_wh e ≠ wh_Diverge ∧ closed e)
+End
+
+
+Definition can_commute_def:
+  can_commute  e e' = ∀f.
+                           ¬ (eval_wh (subst f e) = wh_Diverge ∧ eval_wh (subst f e') = wh_Error) ∧
+                           ¬ (eval_wh (subst f e) = wh_Error ∧ eval_wh (subst f e') = wh_Diverge)
+End
+
+Theorem can_commute_sym:
+  can_commute e e' ⇒ can_commute e' e
+Proof
+  metis_tac [can_commute_def]
+QED
+
+Theorem can_commute_Seq_com:
+  ∀e e'. can_commute e e' ⇒ ∀e''. Seq (Seq e e') e'' ≈ Seq (Seq e' e) e''
+Proof
+  rw [can_commute_def]
+  \\ irule eval_wh_IMP_exp_eq
+  \\ gen_tac
+  \\ ‘eval_wh (subst f e) = wh_Diverge ∨ eval_wh (subst f e) = wh_Error ∨ (eval_wh (subst f e) ≠ wh_Diverge ∧ eval_wh (subst f e) ≠ wh_Error)’ by rw [DISJ_EQ_IMP]
+  \\ ‘eval_wh (subst f e') = wh_Diverge ∨ eval_wh (subst f e') = wh_Error ∨ (eval_wh (subst f e') ≠ wh_Diverge ∧ eval_wh (subst f e') ≠ wh_Error)’ by rw [DISJ_EQ_IMP]
+  \\ rw [subst_def, eval_wh_Seq]
+  \\ fs []
+  \\ metis_tac []
+QED
+
+Theorem is_good_means_can_commute:
+  ∀e e'. is_good e ⇒ can_commute e e'
+Proof
+  fs [is_good_def, can_commute_def]
+QED
+
+Theorem demands_Seq_com:
+  ∀e e'. is_good e ∨ is_good e' ⇒ ∀e''. Seq (Seq e e') e'' ∼ Seq (Seq e' e) e''
+Proof
+  rw [is_good_means_can_commute]
+  \\ irule can_commute_Seq_com
+  \\ fs [is_good_means_can_commute, can_commute_sym]
+QED
+
+Theorem needs_Seq2:
+  (can_commute e (Projs ps e'')) ∧ e' needs (ps, e'')
+  ⇒ (Seq e e') needs (ps, e'')
+Proof
+  rw [DISJ_EQ_IMP]
+  \\ fs [needs_def, Projs_def]
+  \\ qabbrev_tac ‘p = Projs ps e''’
+  \\ irule exp_eq_trans \\ qexists_tac ‘Seq e (Seq p e')’
+  \\ conj_tac
+  >- (irule exp_eq_Prim_cong \\ fs [exp_eq_refl])
+  \\ irule exp_eq_trans \\ qexists_tac ‘Seq (Seq e p) e'’
+  \\ conj_tac
+  >- (‘Seq (Seq e p) e' ∼ Seq e (Seq p e')’ by fs [Seq_assoc]
+      \\ fs [exp_eq_sym])
+  \\ irule exp_eq_trans \\ qexists_tac ‘Seq (Seq p e) e'’
+  \\ fs [Seq_assoc]
+  \\ irule can_commute_Seq_com
+  \\ fs [DISJ_EQ_IMP]
+QED
+
+Theorem demands_Seq2:
+  is_good e ∧ e' demands (ps, v)
+   ⇒ (Seq e e') demands (ps, v)
+Proof
+  metis_tac [is_good_means_can_commute,needs_Var_is_demands, needs_Seq2]
+QED
+
+Theorem needs_If2_no_Diverge:
+  (∀f. eval_wh (subst f ce) ≠ wh_Diverge ∧ eval_wh (subst f e) ≠ wh_Diverge)
+  ∧ te ∼ Seq e te' ∧ ee ∼ Seq e ee'
+  ⇒ If ce te ee ∼ Seq e (If ce te' ee')
+Proof
+  rw []
   \\ irule exp_eq_trans
-  \\ qexists_tac ‘Let w cons (Seq (Projs ps (Proj s (LENGTH xs) (Var w))) e)’
-  \\ conj_tac THEN1
-   (irule exp_eq_App_cong \\ fs [exp_eq_refl]
-    \\ irule exp_eq_Lam_cong \\ fs [exp_eq_refl])
+  \\ qexists_tac ‘If ce (Seq e te') (Seq e ee')’
+  \\ conj_tac
+  >- (irule exp_eq_Prim_cong \\ fs [exp_eq_refl])
+  \\ irule eval_wh_IMP_expeq
+  \\ rw [subst_def, eval_wh_Seq, eval_wh_If]
+  \\ fs []
+QED
+
+Theorem needs_If2:
+  ((is_good ce ∧ (eval_wh ce = wh_True ∨ eval_wh ce = wh_False)) ∨ is_good e') ∧ te needs ([], e') ∧ ee needs ([], e') ⇒ (If ce te ee) needs ([], e')
+Proof
+  rw [is_good_def, needs_def, Projs_def]
   \\ irule exp_eq_trans
-  \\ irule_at Any Let_Seq
-  \\ irule exp_eq_Prim_cong \\ fs [exp_eq_refl,Let_Var]
-  \\ fs [GSYM Projs_def]
+  \\ qexists_tac ‘If ce (Seq e' te) (Seq e' ee)’
+  \\ conj_tac
+  \\ TRY (irule exp_eq_Prim_cong \\ fs [exp_eq_refl])
+  \\ irule eval_wh_IMP_exp_eq
+  \\ rw [subst_def, eval_wh_Seq, eval_wh_If]
+  \\ fs []
+QED
+*)
+
+Theorem needs_projs_reduce:
+  ∀ps ps' e e'. e needs (ps ++ ps', e') ⇒ e needs (ps, e')
+Proof
+  rw [needs_def, double_Projs]
+  \\ qabbrev_tac ‘p = Projs ps e'’
+  \\ irule exp_eq_trans \\ qexists_tac ‘Seq (Seq p (Projs ps' p)) e’
+  \\ conj_tac
+  >- (irule exp_eq_trans \\ first_assum $ irule_at Any
+      \\ irule exp_eq_Prim_cong
+      \\ fs [exp_eq_refl]
+      \\ ‘p needs ([], p)’ by fs [needs_refl]
+      \\ drule needs_Projs
+      \\ rw [needs_def, Projs_def])
+  \\ irule exp_eq_trans \\ qexists_tac ‘Seq p (Seq (Projs ps' p) e)’
+  \\ fs [Seq_assoc]
+  \\ irule exp_eq_Prim_cong
+  \\ fs [exp_eq_refl, exp_eq_sym]
+QED
+
+
+Theorem demands_Projs_empty:
+  ∀ps v. (Projs ps (Var v)) demands ([], v)
+Proof
+  rpt gen_tac
+  \\ ‘(Projs ps (Var v)) demands (ps, v)’ by metis_tac [Projs_def, demands_def, Seq_id, exp_eq_sym]
+  \\ irule $ iffLR needs_Var_is_demands
+  \\ irule needs_projs_reduce
+  \\ fs []
+  \\ rw [needs_Var_is_demands]
+  \\ first_assum $ irule_at Any
+QED
+
+Theorem demands_empty_proj:
+  e demands (ps, v) ⇒ e demands ([], v)
+Proof
+  ‘ps = [] ++ ps’ by rw []
+  \\ rw []
+  \\ metis_tac [needs_projs_reduce, needs_Var_is_demands]
+QED
+
+Theorem demands_projs_reduce:
+  e demands (ps ++ ps', v) ⇒ e demands (ps, v)
+Proof
+  metis_tac [needs_projs_reduce, needs_Var_is_demands]
+QED
+
+Theorem EXISTS_EL:
+  ∀l P. EXISTS P l ⇒ ∃n. n < LENGTH l ∧ P (EL n l)
+Proof
+  Induct
+  \\ fs [EXISTS_DEF]
+  \\ rw []
+  >- (qexists_tac ‘0’
+      \\ fs [])
+  \\ first_x_assum $ dxrule
+  \\ rw []
+  \\ rename1 ‘n < LENGTH l’
+  \\ qexists_tac ‘SUC n’
+  \\ fs []
+QED
+
+Theorem demands_AtomOp:
+  ∀d l op. EXISTS (λe. e demands d) l ⇒ Prim (AtomOp op) l demands d
+Proof
+  gen_tac
+  \\ PairCases_on ‘d’
+  \\ rw [eval_wh_def, eval_wh_to_def, demands_def]
   \\ irule exp_eq_trans
-  \\ irule_at Any Let_Projs
-  \\ fs [Projs_def]
-  \\ irule exp_eq_Projs_cong \\ fs [exp_eq_refl,Let_Var]
-  \\ irule exp_eq_trans
-  \\ irule_at Any exp_eq_Prim_cong \\ fs [PULL_EXISTS]
-  \\ irule_at Any Let_Var
+  \\ irule_at Any exp_eq_Prim_cong
+  \\ drule EXISTS_EL
+  \\ rw []
+  \\ rename1 ‘EL n l ≈ Seq p _’
+  \\ qexists_tac ‘LUPDATE (Seq p (EL n l)) n l’
+(*  \\ qexists_tac ‘GENLIST (λ i. if i = n then Seq p (EL i l) else EL i l) (LENGTH l)’ *)
+  \\ rw [LIST_REL_EL_EQN, EL_LUPDATE]
+  >- (IF_CASES_TAC
+      \\ fs [exp_eq_refl])
+  \\ irule no_err_eval_wh_IMP_exp_eq
+  \\ rw [no_err_eval_wh_def, subst_def, eval_wh_Prim_alt, MAP_MAP_o]
+  \\ qabbrev_tac ‘l2 = LUPDATE (Seq p (EL n l)) n l’
+  >- (qsuff_tac ‘EXISTS error_Atom (MAP (eval_wh o (λa. subst f a)) l2)’
+      >- rw [get_atoms_def]
+      \\ fs [EXISTS_MEM]
+      \\ qexists_tac ‘eval_wh (subst f (EL n l2))’
+      \\ unabbrev_all_tac
+      \\ rw [LUPDATE_MAP, MEM_LUPDATE, EL_LUPDATE]
+      \\ fs [subst_def, eval_wh_Seq])
+  >- (Cases_on ‘EXISTS error_Atom (MAP (eval_wh o (λa. subst f a)) l2)’
+      >- rw [get_atoms_def]
+      \\ qsuff_tac ‘MEM wh_Diverge (MAP (eval_wh ∘ (λa. subst f a)) l2)’
+      >- rw [get_atoms_def]
+      \\ unabbrev_all_tac
+      \\ rw [LUPDATE_MAP, MEM_LUPDATE, subst_def, eval_wh_Seq])
   \\ unabbrev_all_tac
-  \\ fs [Proj_Cons]
+  \\ rw [MAP_GENLIST, Once get_atoms_def]
+  >- (fs [EXISTS_MAP]
+      \\ drule EXISTS_EL
+      \\ rw [EL_LUPDATE]
+      \\ rename1 ‘n2 = n’
+      \\ Cases_on ‘n2 = n’
+      \\ rw []
+      \\ fs [subst_def, eval_wh_Seq]
+      >- (gvs []
+          \\ ‘EXISTS (λx. error_Atom (eval_wh (subst f x))) l’
+            by (fs [EXISTS_MEM]
+                \\ first_x_assum $ irule_at Any
+                \\ fs [EL_MEM])
+          \\ rw [get_atoms_def, EXISTS_MAP])
+      \\ ‘EXISTS (λx. error_Atom (eval_wh (subst f x))) l’
+        by (fs [EXISTS_MEM]
+            \\ first_x_assum $ irule_at Any
+            \\ fs [EL_MEM])
+      \\ rw [get_atoms_def, EXISTS_MAP])
+  \\ fs []
+  \\ ‘¬ EXISTS error_Atom (MAP (eval_wh o (λa. subst f a)) l)’
+    by (rw []
+        \\ fs [EVERY_MEM]
+        \\ rw []
+        \\ fs [MEM_EL]
+        \\ rename1 ‘¬error_Atom (EL n2 _)’
+        \\ Cases_on ‘n2 = n’
+        \\ rw []
+        >- (first_x_assum $ qspecl_then [‘eval_wh (subst f (Seq p (EL n l)))’] assume_tac
+            \\ fs [eval_wh_Seq, subst_def]
+            \\ ‘(if eval_wh (subst f p) = wh_Error then wh_Error
+                 else if eval_wh (subst f p) = wh_Diverge then wh_Diverge
+                 else eval_wh (subst f (EL n l))) = eval_wh (subst f (EL n l))’ by fs []
+            \\ fs [EL_MAP]
+            \\ pop_assum kall_tac
+            \\ pop_assum irule
+            \\ first_assum $ irule_at Any
+            \\ rw [EL_MAP, EL_LUPDATE, subst_def, eval_wh_Seq])
+        \\ first_x_assum irule
+        \\ first_assum $ irule_at Any
+        \\ fs [EL_MAP, EL_LUPDATE])
+  >- (‘MEM wh_Diverge (MAP (eval_wh o (λa. subst f a)) l)’
+        by (fs [MEM_EL]
+            \\ first_assum $ irule_at Any
+            \\ pop_assum kall_tac
+            \\ rename1 ‘EL n2 _’
+            \\ Cases_on ‘n2 = n’
+            >- (fs [EL_MAP, EL_LUPDATE, LUPDATE_MAP, eval_wh_Seq, subst_def]
+                \\ metis_tac [])
+            \\ gvs [LENGTH_LUPDATE, EL_MAP, EL_LUPDATE, eval_wh_Seq, subst_def])
+      \\ rw [get_atoms_def])
+  >- (qsuff_tac ‘MAP (eval_wh o (λa. subst f a)) (LUPDATE (Seq p (EL n l)) n l) = MAP (eval_wh o (λa. subst f a)) l’
+      >- (rw [get_atoms_def]
+          \\ fs [])
+      \\ pop_assum kall_tac
+      \\ pop_assum kall_tac
+      \\ pop_assum kall_tac
+      \\ irule LIST_EQ
+      \\ rw [LENGTH_MAP, LENGTH_LUPDATE, EL_MAP, EL_LUPDATE, eval_wh_Seq, subst_def])
+QED
+
+(*
+Definition fun_demands2_def:
+  f fun_demands (ps,(k:num),(n:num)) ⇒ ∀l hd v. LENGTH l = n ∧ LENGTH hd = k ∧ (l = hd++v::tl) ⇒ Apps f (MAP Var l) demands ([],v)
+End
+*)
+Definition fun_demands_pre_def:
+  fun_demands_pre (k:num) f ps = if k = 0
+                        then ∀n. n ∉ freevars f ⇒ (App f (Var n)) demands (ps, n)
+                        else ∀e. fun_demands_pre (k - 1) (App f e) ps
+End
+
+val _ = set_fixity "fun_demands" (Infixl 478);
+
+Definition fun_demands_def:
+  f fun_demands (ps, k) = fun_demands_pre k f ps
+End
+(*
+Theorem Let_Var_eq:
+  ∀e v. Let v (Var v) e ∼ e
+Proof
+  Induct \\ rw []
+  THEN1 (qsuff_tac ‘v = s ∨ v ≠ s’
+         THEN1 (DISCH_TAC \\ pop_assum DISJ_CASES_TAC
+                THEN1 (rw [] \\ fs [Let_Var])
+                \\ fs [Let_Var2])
+         \\ rw [])
+  THEN1 (irule exp_eq_trans \\ qexists_tac ‘Prim o' (MAP (Let v (Var v)) l)’
+         \\ conj_tac
+         THEN1 fs [Let_Prim]
+QED
+*)
+(*
+Theorem fun_demands_Lam:
+  e demands (ps, v) ⇒ (Lam v e) fun_demands (ps, 0)
+Proof
+  rw [fun_demands_def, fun_demands_pre_def, demands_def]
+  \\ irule exp_eq_trans
+  THEN1 (qexists_tac ‘Let v (Var n) (Seq (Projs ps (Var v)) e)’
+         \\ conj_tac
+         THEN1 (irule exp_eq_App_cong \\ fs [exp_eq_refl]
+                \\ irule exp_eq_Lam_cong \\ fs [])
+         \\ irule exp_eq_trans \\ qexists_tac ‘Seq (Let v (Var n) (Projs ps (Var v))) (Let v (Var n) e)’
+         \\ conj_tac
+         THEN1 fs [Let_Seq]
+         \\ irule exp_eq_Prim_cong
+         \\ fs [exp_eq_refl]
+         \\ irule exp_eq_trans \\ qexists_tac ‘Projs ps (Let v (Var n) (Var v))’
+         \\ conj_tac
+         THEN1 fs [Let_Projs]
+         \\ irule exp_eq_Projs_cong \\ fs [Let_Var])
+  \\ qexists_tac ‘e’ \\ conj_tac
+  THEN1 fs [Let_Var_eq]
+  \\ irule exp_eq_trans \\ qexists_tac ‘Seq (Projs ps (Var n)) e’
+  THEN1 fs []
+  \\ irule exp_eq_Prim_cong \\ fs [exp_eq_refl]
+QED
+
+Theorem fun_demands_Let:
+  ∀f. (f fun_demands (ps, k) ⇒ ∀e v. (App (Lam v f) e) fun_demands (ps, k))
+Proof
+  rw [fun_demands_def, Once fun_demands_pre_def, demands_def]
+  THEN1 (rw [fun_demands_pre_def]
+   \\ rw [demands_def]
+   \\ irule exp_eq_trans \\ qexists_tac ‘Let v e (App f (Var n))’
+   \\ conj_tac
+   THEN1 (irule exp_eq_trans \\ qexists_tac ‘App (Let v e f) (Let v e (Var n))’
+    \\ conj_tac
+    THEN1 (irule exp_eq_App_cong \\ fs [exp_eq_refl])
+*)
+
+Theorem exp_eq_Apps_cong:
+  ∀l l' b e e'. LIST_REL (λx y. (x ≅? y) b) l l' ⇒ (e ≅? e') b ⇒ (Apps e l ≅? Apps e' l') b
+Proof
+  Induct
+  \\ fs [Apps_def]
+  \\ rw [Apps_def]
+  \\ fs [Apps_def]
+  \\ first_x_assum $ irule
+  \\ fs [exp_eq_App_cong]
+QED
+
+Theorem exp_eq_Lams_cong:
+  ∀l e e' b. (e ≅? e') b ⇒ (Lams l e ≅? Lams l e') b
+Proof
+  Induct
+  \\ rw [Lams_def]
+  \\ fs [exp_eq_Lam_cong]
+QED
+
+Theorem Apps_demands:
+  ∀el d e. e demands d ⇒ Apps e el demands d
+Proof
+  Induct
+  \\ fs [Apps_def]
+  \\ gen_tac
+  \\ rw []
+  \\ first_x_assum irule
+  \\ fs [demands_App]
 QED
 
 Datatype:
   ctxt = Nil
-       | Append ctxt ctxt
-       | Bind string exp ctxt
-       | RecBind (string # exp) ctxt
+       | IsFree string ctxt
+       | Bind string exp ctxt ctxt
+       | RecBind ((string # exp) list) ctxt
+End
+
+Definition ctxt_size_def:
+  ctxt_size Nil = 0n ∧
+  ctxt_size (IsFree s ctxt) = 1 + ctxt_size ctxt ∧
+  ctxt_size (Bind s e ctxt tl) = 1 + list_size char_size s +  exp_size e + ctxt_size ctxt + ctxt_size tl ∧
+  ctxt_size (RecBind sel ctxt) = 1 + exp1_size sel + ctxt_size ctxt
+End
+
+Definition subst_ctxt_def:
+  (subst_ctxt ctxt (App f e) = App (subst_ctxt ctxt f) (subst_ctxt ctxt e)) ∧
+  (subst_ctxt  ctxt (Prim op l) = Prim op (MAP (subst_ctxt ctxt) l)) ∧
+  (subst_ctxt ctxt (Lam v e) = Lam v (subst_ctxt (IsFree v ctxt) e)) ∧
+  (subst_ctxt Nil (Var n) = Var n) ∧
+  (subst_ctxt (IsFree v ctxt) (Var n) = if n = v
+                                        then Var n
+                                        else subst_ctxt ctxt (Var n)) ∧
+  (subst_ctxt (Bind v exp ctxt tl) (Var n) = if n = v
+                                         then subst_ctxt ctxt exp
+                                         else subst_ctxt tl (Var n)) ∧
+  (subst_ctxt (RecBind nel ctxt) (Var n) = if MEM n (MAP FST nel)
+                                                then Var n
+                                                else subst_ctxt ctxt (Var n)) ∧
+  (subst_ctxt ctxt (Letrec nel e) = Letrec nel (subst_ctxt (RecBind nel ctxt) e))
+Termination
+  WF_REL_TAC ‘inv_image ($< LEX $<) (λ(c,e).(exp_size e + ctxt_size c, exp_size e))’
+  \\ rw [ctxt_size_def] \\ fs []
 End
 
 Inductive find: (* i i o o *)
 [find_Bottom:]
-  (∀e c.
+  (∀e (c:ctxt).
     find e c {} e) ∧
 [find_Seq:]
-  (∀e c p ds v.
-    find e c ds e ∧ (p,v) ∈ ds ⇒
-    find e c ds (Seq (Var v) e))
+  (∀e e' c (p:(string#num) list) ds v.
+    find e c ds e' ∧ (p,v) ∈ ds ⇒
+    find e c ds (Seq (Var v) e')) ∧
+[find_Seq2:]
+  (∀e e' e2 e2' c ds ds2.
+     find e c ds e' ∧ find e2 c ds2 e2' ⇒
+     find (Seq e e2) c (ds ∪ ds2) (Seq e' e2')) ∧
+[find_If:]
+  (∀ec et ee ec' et' ee' c dsc dst dse.
+     find ec c dsc ec' ∧
+     find et c dst et' ∧
+     find ee c dse ee' ⇒
+     find (If ec et ee) c (dsc ∪ (dst ∩ dse)) (If ec' et' ee')) ∧
+[find_Var:]
+  (∀n c. find (Var n) c {([],n)} (Var n)) ∧
+[find_App:]
+  (∀f f' e e' c ds ds2.
+     find f c ds f' ∧
+     find e c ds2 e' ⇒
+     find (App f e) c ds (App f' e')) ∧
+[find_Apps:]
+  (∀f f' el el' c ds.
+     LIST_REL (λe e'. ∃ds. find e c ds e') el el' ∧
+     find f c ds f' ⇒ find (Apps f el) c ds (Apps f' el')) ∧
+[find_Prim:]
+  (∀c el el' ope.
+     LENGTH el = LENGTH el' ∧ (∀k. k < LENGTH el ⇒ ∃ds. find (EL k el) c ds (EL k el') )
+     ⇒ find (Prim ope el) c {} (Prim ope el')) ∧
+[find_Prim1:]
+  (∀c el el' ope ds.
+     LENGTH el = LENGTH el' ∧
+     (∀k. k < LENGTH el ⇒ ∃ds'. find (EL k el) c ds' (EL k el')) (* Rewritte with LIST_REL *)
+     ∧ find (EL 0 el) c ds (EL 0 el') ∧ el ≠ [] ∧ well_formed ope el ⇒ find (Prim ope el) c ds (Prim ope el')) ∧
+[find_Prim_Fail:]
+  (∀c el ope.
+     ¬ (well_written ope el) ⇒ find (Prim ope el) c {} Fail) ∧
+[find_Proj:]
+  (∀e e' n i c ds.
+     find e c ds e' ⇒ find (Proj n i e) c ds (Proj n i e')) ∧
+[find_IsEq:]
+  (∀e e' n i c ds.
+     find e c ds e' ⇒ find (IsEq n i e) c ds (IsEq n i e')) ∧
+[find_Atom:]
+  (∀el dsl el' c op.
+     LENGTH dsl = LENGTH el' ∧
+     LIST_REL (λe (ds, e'). find e c ds e') el (ZIP (dsl, el')) ⇒
+     find (Prim (AtomOp op) el) c (BIGUNION (set dsl)) (Prim (AtomOp op) el')) ∧
+[find_Subset:]
+  (∀e e' c ds ds'.
+     find e c ds e' ∧ (∀ps v. (ps, v) ∈ ds' ⇒ ∃ps'. (ps++ps', v) ∈ ds) ⇒ find e c ds' e') ∧
+[find_Let:]
+  (∀e e' e2 e2' ds ds' c v.
+     find e c ds e' ∧ find e2 (Bind v e c c) ds' e2'
+     ∧ (∀ps. (ps, v) ∉ ds')
+     ⇒ find (Let v e e2) c ds' (Let v e' e2')) ∧
+[find_Let2:]
+  (∀ e e' e2 e2' ds ds' ds'' c v ps.
+     find e c ds e' ∧ find e2 (Bind v e c c) ds' e2'
+     ∧ (ps,v) ∈ ds'
+     ∧ (∀ps' v'. (ps', v') ∈ ds'' ⇒ ((ps', v') ∈ ds' ∧ v' ≠ v) ∨ (ps', v') ∈ ds)
+     ⇒ find (Let v e e2) c ds'' (Let v e' e2')) ∧
+[find_Lam:]
+  (∀e e' c ds v.
+     find e c ds e' ⇒ find (Lam v e) c {} (Lam v e')) ∧
+[find_Lams:]
+  (∀e e' c ds vl.
+     find e (FOLDL (λc n. IsFree n c) c vl) ds e' ⇒ find (Lams vl e) c {} (Lams vl e')) ∧
+[find_Eq:]
+  (∀e e' c. e ≈ e' ⇒ find e c {} e') ∧
+[find_Letrec:]
+  (∀e e' ds c b b'. LIST_REL (λ(n1, e1) (n2, e2). n1 = n2 ∧ e1 ≈ e2) b b' ∧ find e (RecBind b c) ds e' ⇒ find (Letrec b e) c {} (Letrec b e'))
 End
 
-(*
 
+fun apply_to_first_n 0 tac = ALL_TAC
+  | apply_to_first_n n tac = apply_to_first_n (n-1) tac >- tac;
+
+Theorem find_soundness_lemma:
+  ∀e c ds e'. find e c ds e'  ⇒
+                e ≈ e' ∧
+                (∀d. d ∈ ds ⇒ e demands d)
+Proof
+  Induct_on ‘find’
+  \\ rpt conj_tac
+  \\ rpt gen_tac
+  >- fs [exp_eq_refl] (* find_Bottom *)
+  >~[‘e ≈ Seq (Var v) e2’] (* find_Seq *)
+  >- (strip_tac
+      \\ strip_tac
+      \\ fs []
+      \\ first_x_assum $ drule
+      \\ rw []
+      \\ dxrule_then assume_tac demands_empty_proj
+      \\ fs [demands_def, Projs_def]
+      \\ irule exp_eq_trans
+      \\ first_assum $ irule_at Any
+      \\ irule exp_eq_Prim_cong
+      \\ fs [exp_eq_refl])
+  >~[‘Seq e e2 ≈ Seq e' e2'’] (* find_Seq2 *)
+  >- (rw []
+      \\ fs [exp_eq_Prim_cong, demands_Seq, demands_Seq2])
+  >~[‘If ec et ee ≈ If ec' et' ee'’]
+  >- (rw []
+      \\ fs [demands_If, demands_If2, exp_eq_Prim_cong])
+  >~[‘Var n ≈ Var n’] (* find_Var *)
+  >- fs [exp_eq_refl, demands_Var]
+  >~[‘App f e ≈ App f' e'’] (* find_App *)
+  >- (rw []
+      \\ fs [exp_eq_App_cong, demands_App])
+  >~[‘Apps e el' ≈ Apps e' el''’]
+  >- (rw []
+      \\ fs [Apps_demands]
+      \\ irule exp_eq_Apps_cong
+      \\ fs [LIST_REL_EL_EQN]
+      \\ rw []
+      \\ first_x_assum $ qspecl_then [‘n’] assume_tac
+      \\ metis_tac [])
+  >~[‘Proj n i e ≈ Proj n i e'’] (* find_Proj *)
+  >- (strip_tac
+      \\ fs [exp_eq_Prim_cong, demands_Proj])
+  >~[‘IsEq n i e ≈ IsEq n i e'’] (* find_IsEq *)
+  >- (rw []
+      \\ fs [exp_eq_Prim_cong, demands_IsEq])
+  >~[‘Prim (AtomOp op) el1 ≈ Prim (AtomOp op) el2’]
+  >- (rw []
+      >- (irule exp_eq_Prim_cong
+          \\ fs [LIST_REL_EL_EQN]
+          \\ rw []
+          \\ rename1 ‘n < LENGTH _’
+          \\ first_x_assum $ qspecl_then [‘n’] assume_tac
+          \\ gvs [EL_ZIP])
+      \\ fs [LIST_REL_EL_EQN, MEM_EL]
+      \\ rename1 ‘ds = EL n dsl’
+      \\ first_x_assum $ qspecl_then [‘n’] assume_tac
+      \\ irule demands_AtomOp
+      \\ gvs [EL_ZIP, EXISTS_MEM]
+      \\ pop_assum $ irule_at Any
+      \\ fs [MEM_EL]
+      \\ first_x_assum $ irule_at Any
+      \\ fs [])
+  >>~[‘Prim ope el1 ≈ Prim ope el2’] (* find_Prim *)
+  >- (rw []
+      \\ irule exp_eq_Prim_cong
+      \\ rw [LIST_REL_EL_EQN, EL_MAP]
+      \\ rename1 ‘EL n _’
+      \\ ‘n < LENGTH el1’ by fs []
+      \\ first_x_assum drule
+      \\ rw [])
+  >- (rw [] (* find_Prim1 *)
+      >- (irule exp_eq_Prim_cong
+          \\ rw [LIST_REL_EL_EQN, EL_MAP]
+          \\ rename1 ‘EL n _’
+          \\ ‘n < LENGTH el1’ by fs []
+          \\ first_x_assum drule
+          \\ rw []
+          \\ fs [])
+      \\ rw []
+      \\ last_x_assum dxrule
+      \\ rw []
+      \\ Cases_on ‘el1’
+      \\ fs [demands_Prim])
+  >~[‘Prim ope el1 ≈ Fail’] (* find_Prim_Fail *)
+  >- (rw []
+      \\ fs [not_well_written_is_fail])
+  >>~[‘Let v e e2 ≈ Let v e' e2'’] (* find_Let *)
+  >- (rw []
+      \\ fs [exp_eq_App_cong, exp_eq_Lam_cong]
+      \\ rename1 ‘_ demands d’
+      \\ PairCases_on ‘d’
+      \\ irule demands_Let2
+      \\ ‘d1 = v ∨ d1 ≠ v’ by fs []
+      \\ fs []
+      \\ last_x_assum irule
+      \\ first_x_assum $ irule_at Any)
+  >- (rw []
+      \\ fs [exp_eq_App_cong, exp_eq_Lam_cong]
+      \\ rename1 ‘_ demands d’
+      \\ PairCases_on ‘d’
+      \\ first_x_assum dxrule
+      \\ rw []
+      >- fs [demands_Let2]
+      \\ irule demands_Let1
+      \\ fs []
+      \\ first_x_assum drule
+      \\ rw []
+      \\ drule demands_empty_proj
+      \\ fs [])
+  >- (rw [] (* find_Subset *)
+      \\ rename1 ‘e demands d’ \\ PairCases_on ‘d’
+      \\ first_x_assum drule
+      \\ rw []
+      \\ first_x_assum drule
+      \\ rw []
+      \\ drule demands_projs_reduce
+      \\ fs [])
+  >- (rw [] (* find_Lam *)
+      \\ fs [exp_eq_Lam_cong])
+  >- (rw []
+      \\ fs [exp_eq_Lams_cong])
+  >- (rw []
+      \\ fs [])
+  >- (rw []
+      \\ fs [exp_eq_Letrec_cong, exp_eq_l_refl])
+QED
+
+Theorem find_soundness:
+  find e Nil ds e' ⇒ e ≈ e'
+Proof
+  rw []
+  \\ dxrule find_soundness_lemma
+  \\ fs []
+QED
+
+Datatype:
+  demands_tree = DemandNode bool (((string # num) # demands_tree) list)
+End
+
+Definition dt_to_set_def:
+  dt_to_set (DemandNode T []) ps v = {(ps,v)} ∧
+  dt_to_set (DemandNode F []) ps v = {} ∧
+  dt_to_set (DemandNode b ((p, dt)::tl)) ps v = (dt_to_set dt (ps ++ [p]) v) ∪ (dt_to_set (DemandNode b tl) ps v)
+End
+
+Definition merge_dt_def:
+  merge_dt (DemandNode b1 f1) (DemandNode b2 []) = DemandNode (b1 ∨ b2) f1 ∧
+  merge_dt (DemandNode b1 []) (DemandNode b2 f2) = DemandNode (b1 ∨ b2) f2 ∧
+  merge_dt (DemandNode b1 ((id1,dt1)::tl1)) (DemandNode b2 ((id2,dt2)::tl2)) =
+  if id1 = id2
+  then
+    case merge_dt (DemandNode b1 tl1) (DemandNode b2 tl2) of
+    | DemandNode b3 tl3 => DemandNode b3 ((id1, merge_dt dt1 dt2)::tl3) (* id1 = id2 *)
+  else
+    if FST id1 < FST id2 ∨ (FST id1 = FST id2 ∧ SND id1 < SND id2)
+    then
+      case merge_dt (DemandNode b1 tl1) (DemandNode b2 ((id2,dt2)::tl2)) of
+      | DemandNode b3 tl3 => DemandNode b3 ((id1, dt1)::tl3) (* id1 < id2 *)
+    else
+      case merge_dt (DemandNode b1 ((id1,dt1)::tl1)) (DemandNode b2 tl2) of
+      | DemandNode b3 tl3 => DemandNode b3 ((id2, dt2)::tl3) (* id2 < id1 *)
+End
+
+Definition find_function_def:
+  find_function (Var v) c = ((FEMPTY : (string |-> demands_tree)) |+ (v, DemandNode T []), Var v) ∧
+  (find_function (If ce te ee) c =
+   let (cd, ce') = find_function ce c in
+     let (td, te') = find_function te c in
+       let (ed, ee') = find_function ee c in
+         (cd, If ce' te' ee')) ∧
+  (find_function (Prim If _) c = (FEMPTY, Fail)) ∧
+  (find_function (Proj s i e) c =
+   let (d, e') = find_function e c in
+     (d, Proj s i e')) ∧
+  (find_function (Prim (Proj s i) _) c = (FEMPTY, Fail)) ∧
+  (find_function (IsEq s i e) c =
+   let (d, e') = find_function e c in
+     (d, IsEq s i e')) ∧
+  (find_function (Prim (IsEq s i) _) c = (FEMPTY, Fail)) ∧
+  (find_function (Seq e1 e2) c =
+   let (d1, e1') = find_function e1 c in
+     let (d2, e2') = find_function e2 c in
+       (d1, Seq e1' e2')) ∧
+  (find_function (Prim Seq _) c = (FEMPTY, Fail)) ∧
+  (find_function (Prim op l) c =
+  (FEMPTY, Prim op (MAP (λe. SND (find_function e c)) l))) ∧
+  (find_function (App (Lam v e2) e) c = let (d, e') = find_function e c in
+                                          let (d2, e2') = find_function e2 (Bind v e c c) in
+                                           case FLOOKUP d2 v of
+                                             | NONE => (d2, App (Lam v e2') e')
+                                             | SOME s => (FMERGE merge_dt d (d2 \\ v), Let v e' (Seq (Var v) e2'))) ∧
+  (find_function (App f e) c = let (d, f') = find_function f c in
+                                 let (_, e') = find_function e c in
+                                   (d, App f' e')) ∧
+  find_function e c = ((FEMPTY, e) : (string |-> demands_tree) # exp)
+Termination
+  WF_REL_TAC ‘measure (exp_size o FST)’
+  \\ rw [] \\ fs []
+  \\ assume_tac exp_size_lemma
+  \\ fs []
+  \\ first_x_assum dxrule
+  \\ fs []
+End
+
+Theorem exp_size_cmp_exp3_size:
+  ∀l e. MEM e l ⇒ exp_size e < exp3_size l
+Proof
+  fs [exp_size_lemma]
+QED
+
+Definition demands_tree_size_def:
+  demands_tree_size (DemandNode b []) = 1 ∧
+  demands_tree_size (DemandNode b ((v,dt)::tl)) = 1 + demands_tree_size dt + demands_tree_size (DemandNode b tl)
+End
+
+Theorem dt_to_set_union:
+  ∀l b p v. dt_to_set (DemandNode T l) p v = {(p, v)} ∪ dt_to_set (DemandNode b l) p v
+Proof
+  Induct
+  \\ rw [dt_to_set_def]
+  >- (rename1 ‘DemandNode b []’
+      \\ Cases_on ‘b’
+      \\ rw [dt_to_set_def])
+  \\ rename1 ‘DemandNode b (hd::tl)’
+  \\ Cases_on ‘hd’
+  \\ rw [dt_to_set_def]
+  \\ metis_tac [UNION_COMM, UNION_ASSOC]
+QED
+
+Theorem merge_dt_is_set_union:
+  ∀dt1 dt2 p v. dt_to_set (merge_dt dt1 dt2) p v = (dt_to_set dt1 p v) ∪ (dt_to_set dt2 p v)
+Proof
+  Induct using demands_tree_size_ind
+  >- (Cases
+      \\ Cases
+      \\ rename1 ‘DemandNode b2 l’
+      \\ Cases_on ‘b2’
+      \\ Cases_on ‘l’
+      \\ rw [merge_dt_def, dt_to_set_def]
+      \\ fs [dt_to_set_union])
+  \\ Induct using demands_tree_size_ind
+  >- (rpt gen_tac
+      \\ rename1 ‘DemandNode b2 []’
+      \\ Cases_on ‘b2’
+      \\ rw [dt_to_set_def, merge_dt_def]
+      \\ metis_tac [dt_to_set_union, UNION_COMM, UNION_ASSOC])
+  \\ rpt gen_tac
+  \\ rename1 ‘merge_dt (DemandNode b1 ((v1,dt1)::tl1)) (DemandNode b2 ((v2,dt2)::tl2))’
+  \\ rw [merge_dt_def]
+  >- (qabbrev_tac ‘dt3 = merge_dt (DemandNode b1 tl1) (DemandNode b2 tl2)’
+      \\ Cases_on ‘dt3’
+      \\ rw [dt_to_set_def]
+      \\ unabbrev_all_tac
+      \\ metis_tac [UNION_COMM, UNION_ASSOC])
+  >- (qabbrev_tac ‘dt3 = merge_dt (DemandNode b1 tl1) (DemandNode b2 ((v2,dt2)::tl2))’
+      \\ Cases_on ‘dt3’
+      \\ rw [dt_to_set_def]
+      \\ unabbrev_all_tac
+      \\ metis_tac [UNION_COMM, UNION_ASSOC, dt_to_set_def])
+  >- (qabbrev_tac ‘dt3 = merge_dt (DemandNode b1 tl1) (DemandNode b2 ((v2,dt2)::tl2))’
+      \\ Cases_on ‘dt3’
+      \\ rw [dt_to_set_def]
+      \\ unabbrev_all_tac
+      \\ metis_tac [UNION_COMM, UNION_ASSOC, dt_to_set_def])
+  \\ qabbrev_tac ‘dt3 = merge_dt (DemandNode b1 ((v1, dt1)::tl1)) (DemandNode b2 tl2)’
+  \\ Cases_on ‘dt3’
+  \\ rw [dt_to_set_def]
+  \\ unabbrev_all_tac
+  \\ metis_tac [UNION_COMM, UNION_ASSOC]
+QED
+
+Theorem find_function_soundness_lemma:
+  ∀ e c d e' b.
+    find_function e c = (d, e') ⇒
+    ∃ds. find e c ds e' ∧
+         (∀s ps. (ps, s) ∈ ds ⇒ ∃dt. FLOOKUP d s = SOME dt ∧ (ps, s) ∈ dt_to_set dt [] s) ∧
+         (∀s. s ∈ FDOM d ⇒ ∃ps. (ps, s) ∈ ds)
+Proof
+  completeInduct_on ‘exp_size e’
+  \\ rename1 ‘k = exp_size _’
+  \\ gen_tac \\ Cases_on ‘e’
+  \\ fs [exp_size_def]
+  >- (rw [find_function_def] (* Var v *)
+      \\ rename1 ‘(v, DemandNode T [])’
+      \\ qexists_tac ‘{([], v)}’
+      \\ fs [find_Var]
+      \\ qexists_tac ‘DemandNode T []’
+      \\ rw [dt_to_set_def, FLOOKUP_UPDATE])
+  >- (rw [] (* Prim op l *)
+      \\ rename1 ‘Prim op es’
+      \\ Cases_on ‘es’
+      >- (Cases_on ‘op’ (* Prim op [] *)
+          \\ fs [find_function_def]
+          \\ qexists_tac ‘{}’
+          \\ fs [find_Bottom]
+          \\ irule find_Prim_Fail
+          \\ fs [well_written_def])
+      \\ rename1 ‘h::t’
+      \\ Cases_on ‘op’ >~[‘Prim (Cons s) (h::tl)’]
+      >- (fs [find_function_def]
+          \\ qabbrev_tac ‘es = h::tl’
+          \\ qexists_tac ‘{}’
+          \\ fs []
+          \\ rw []
+          \\ irule find_Prim
+          \\ rw [] >~[‘LENGTH _ = _’] >- (unabbrev_all_tac \\ fs [])
+          \\ rename1 ‘EL k' es’
+          \\ ‘exp_size (EL k' es) < exp3_size es + (op_size (Cons s) + 1)’ by
+            (‘exp_size (EL k' es) < exp3_size es’ by
+               (irule exp_size_cmp_exp3_size
+                \\ fs [MEM_EL]
+                \\ qexists_tac ‘k'’
+                \\ fs []
+                \\ unabbrev_all_tac
+                \\ fs [])
+             \\ fs [])
+          \\ first_x_assum dxrule
+          \\ rw []
+          \\ ‘exp_size (EL k' es) = exp_size (EL k' es)’ by fs []
+          \\ first_x_assum dxrule
+          \\ qabbrev_tac ‘de = find_function (EL k' es) c’
+          \\ PairCases_on ‘de’
+          \\ rw []
+          \\ ‘de1 = EL k' (MAP (λe. SND (find_function e c)) es)’ by
+            fs [EL_MAP]
+          \\ fs[]
+          \\ unabbrev_all_tac
+          \\ fs []
+          \\ first_x_assum drule
+          \\ rw []
+          \\ first_x_assum $ irule_at Any)
+      >- (Cases_on ‘t’
+          >- (fs [find_function_def] (* Prim If [e] *)
+              \\ qexists_tac ‘{}’
+              \\ fs []
+              \\ rw []
+              \\ fs [find_Prim_Fail, well_written_def])
+          \\ rename1 ‘h::h1::t’
+          \\ Cases_on ‘t’
+          >- (fs [find_function_def] (* Prim If [e, e'] *)
+              \\ qexists_tac ‘{}’
+              \\ rw []
+              \\ fs [find_Prim_Fail, well_written_def])
+          \\ rename1 ‘ce::te::ee::t’
+          \\ Cases_on ‘t’
+          >- (fs [find_function_def] (* If _ _ _ *)
+              \\ qabbrev_tac ‘ce' = find_function ce c’ \\ PairCases_on ‘ce'’
+              \\ qabbrev_tac ‘te' = find_function te c’ \\ PairCases_on ‘te'’
+              \\ qabbrev_tac ‘ee' = find_function ee c’ \\ PairCases_on ‘ee'’
+              \\ fs []
+              \\ first_assum $ qspecl_then [‘exp_size ce’] assume_tac
+              \\ first_assum $ qspecl_then [‘exp_size te’] assume_tac
+              \\ first_assum $ qspecl_then [‘exp_size ee’] assume_tac
+              \\ fs [exp_size_def]
+              \\ last_x_assum $ qspecl_then [‘ce’] assume_tac
+              \\ last_x_assum $ qspecl_then [‘te’] assume_tac
+              \\ last_x_assum $ qspecl_then [‘ee’] assume_tac
+              \\ fs []
+              \\ first_x_assum dxrule
+              \\ first_x_assum dxrule
+              \\ first_x_assum dxrule
+              \\ rw []
+              \\ qexists_tac ‘ds’
+              \\ fs []
+              \\ irule find_Subset
+              \\ irule_at Any find_If
+              \\ first_x_assum $ irule_at Any
+              \\ first_x_assum $ irule_at Any
+              \\ first_x_assum $ irule_at Any
+              \\ rw []
+              \\ qexists_tac ‘[]’
+              \\ fs [])
+          \\ fs [find_function_def]
+          \\ qexists_tac ‘{}’
+          \\ rw []
+          \\ fs [find_Prim_Fail, well_written_def])
+      >- (Cases_on ‘t’ (* IsEq *)
+          \\ fs [find_function_def]
+          >- (qabbrev_tac ‘ff = find_function h c’
+              \\ PairCases_on ‘ff’
+              \\ first_x_assum $ qspecl_then [‘exp_size h’] assume_tac
+              \\ fs [exp_size_def]
+              \\ pop_assum $ qspecl_then [‘h’] assume_tac
+              \\ fs []
+              \\ pop_assum dxrule
+              \\ rw []
+              \\ irule_at Any find_IsEq
+              \\ first_x_assum $ irule_at Any
+              \\ fs [])
+          \\ qexists_tac ‘{}’
+          \\ fs [find_Prim_Fail, well_written_def])
+      >- (Cases_on ‘t’ (* Proj *)
+          \\ fs [find_function_def]
+          >- (qabbrev_tac ‘ff = find_function h c’
+              \\ PairCases_on ‘ff’
+              \\ first_x_assum $ qspecl_then [‘exp_size h’] assume_tac
+              \\ fs [exp_size_def]
+              \\ pop_assum $ qspecl_then [‘h’] assume_tac
+              \\ fs []
+              \\ pop_assum dxrule
+              \\ rw []
+              \\ irule_at Any find_Proj
+              \\ first_x_assum $ irule_at Any
+              \\ fs [])
+          \\ qexists_tac ‘{}’
+          \\ fs [find_Prim_Fail, well_written_def])
+      >- (qabbrev_tac ‘l = h::t’ (* AtomOp *)
+          \\ qexists_tac ‘{}’
+          \\ fs [find_function_def]
+          \\ rw []
+          \\ irule find_Prim
+          \\ rw []
+          \\ rename1 ‘n < LENGTH l’
+          \\ ‘exp_size (EL n l) < exp3_size l + (op_size (AtomOp a) + 1)’ by
+            ( ‘exp_size (EL n l) < exp3_size l’ by fs [exp_size_cmp_exp3_size, EL_MEM]
+              \\ fs [])
+          \\ first_x_assum $ qspecl_then [‘exp_size (EL n l)’] assume_tac
+          \\ pop_assum $ dxrule_then assume_tac
+          \\ pop_assum $ qspecl_then [‘EL n l’] assume_tac
+          \\ fs []
+          \\ qabbrev_tac ‘p = find_function (EL n l) c’
+          \\ PairCases_on ‘p’
+          \\ fs []
+          \\ rw [EL_MAP]
+          \\ first_x_assum dxrule
+          \\ rw []
+          \\ first_x_assum $ irule_at Any)
+      >- (Cases_on ‘t’ (* Seq *)
+          >- (fs [find_function_def]
+              \\ qexists_tac ‘{}’
+              \\ fs [find_Prim_Fail, well_written_def])
+          \\ rename1 ‘h0::h1::tl’
+          \\ Cases_on ‘tl’
+          >- (first_assum $ qspecl_then [‘exp_size h0’] assume_tac
+              \\ first_x_assum $ qspecl_then [‘exp_size h1’] assume_tac
+              \\ fs [exp_size_def]
+              \\ first_x_assum $ qspecl_then [‘h1’] assume_tac
+              \\ first_x_assum $ qspecl_then [‘h0’] assume_tac
+              \\ fs []
+              \\ fs [find_function_def]
+              \\ qabbrev_tac ‘f1 = find_function h1 c’
+              \\ PairCases_on ‘f1’
+              \\ qabbrev_tac ‘f0 = find_function h0 c’
+              \\ PairCases_on ‘f0’
+              \\ fs []
+              \\ first_x_assum dxrule
+              \\ first_x_assum dxrule
+              \\ rw []
+              \\ irule_at Any find_Subset
+              \\ irule_at Any find_Seq2
+              \\ first_x_assum $ irule_at Any
+              \\ first_x_assum $ irule_at Any
+              \\ qexists_tac ‘ds'’
+              \\ rw []
+              \\ fs []
+              \\ qexists_tac ‘[]’
+              \\ fs [])
+          \\ fs [find_function_def]
+          \\ qexists_tac ‘{}’
+          \\ fs [find_Prim_Fail, well_written_def]))
+  >- (rw [] (* App *)
+      \\ rename1 ‘App f e’
+      \\ first_assum $ qspecl_then [‘exp_size f’] assume_tac
+      \\ fs []
+      \\ pop_assum $ qspecl_then [‘f’] assume_tac
+      \\ qabbrev_tac ‘e1p = find_function f c’
+      \\ PairCases_on ‘e1p’
+      \\ fs []
+      \\ first_x_assum drule
+      \\ strip_tac
+      \\ Cases_on ‘f’ >~[‘Let s e e2’]
+      >- (
+       first_assum $ qspecl_then [‘exp_size e’] assume_tac
+       \\ first_x_assum $ qspecl_then [‘exp_size e2’] assume_tac
+       \\ fs [exp_size_def, find_function_def]
+       \\ qabbrev_tac ‘ep = find_function e c’
+       \\ PairCases_on ‘ep’
+       \\ qabbrev_tac ‘e2p = find_function e2 (Bind s e c c)’
+       \\ PairCases_on ‘e2p’
+       \\ last_x_assum $ qspecl_then [‘e’] assume_tac
+       \\ last_x_assum $ qspecl_then [‘e2’] assume_tac
+       \\ fs []
+       \\ first_x_assum dxrule
+       \\ first_x_assum dxrule
+       \\ rw []
+       \\ rename1 ‘find e2 _ ds2 _’
+       \\ rename1 ‘find e _ ds1 _’
+       \\ ‘s ∈ FDOM e2p0 ∨ s ∉ FDOM e2p0’ by fs []
+       \\ fs [FLOOKUP_DEF]
+       \\ rw []
+       >- (
+         irule_at Any find_Let2
+         \\ first_x_assum $ irule_at Any
+         \\ irule_at Any find_Seq
+         \\ first_x_assum $ irule_at Any
+         \\ first_assum $ dxrule
+         \\ rw []
+         \\ first_assum $ irule_at Any
+         \\ first_x_assum $ irule_at Any
+         \\ ‘∃ds'''. ∀ps v. (ps, v) ∈ ds''' ⇔ ((ps, v) ∈ ds2 ∧ v ≠ s) ∨ (ps, v) ∈ ds1’ by
+            (qexists_tac ‘ds1 ∪ BIGUNION (IMAGE (λ(ps,v). if v = s then {} else {(ps,v)}) ds2)’
+             \\ rw []
+             \\ eq_tac
+             \\ rw []
+             \\ fs []
+             >- (rename1 ‘p ∈ ds2’
+                 \\ PairCases_on ‘p’
+                 \\ fs []
+                 \\ ‘p1 = s ∨ p1 ≠ s’ by fs []
+                 \\ fs [])
+             \\ rw [DISJ_EQ_IMP]
+             \\ qexists_tac ‘{(ps, v)}’
+             \\ fs []
+             \\ first_x_assum $ irule_at Any
+             \\ fs [])
+         \\ qexists_tac ‘ds'''’
+         \\ fs []
+         \\ rw []
+         \\ first_x_assum dxrule
+         \\ fs []
+         >- (rw [FMERGE_DEF]
+             >- (qsuff_tac ‘FLOOKUP (e2p0 \\ s) s' = FLOOKUP e2p0 s'’
+                 >- rw [FLOOKUP_DEF]
+                 \\ fs [DOMSUB_FLOOKUP_NEQ])
+             \\ fs [merge_dt_is_set_union]
+             \\ qsuff_tac ‘FLOOKUP (e2p0 \\ s) s' = FLOOKUP e2p0 s'’
+             >- rw [FLOOKUP_DEF]
+             \\ fs [DOMSUB_FLOOKUP_NEQ])
+         >- rw [FMERGE_DEF, merge_dt_is_set_union]
+         >- (rw []
+             \\ qexists_tac ‘ps’
+             \\ fs [])
+         \\ rw []
+         \\ qexists_tac ‘ps’
+         \\ fs [])
+       \\ irule_at Any find_Let
+       \\ last_x_assum $ irule_at Any
+       \\ last_x_assum $ irule_at Any
+       \\ fs []
+       \\ rw []
+       >- (strip_tac
+           \\ first_x_assum dxrule
+           \\ fs [])
+       \\ first_assum drule
+       \\ fs [])
+      \\ fs [find_function_def]
+      \\ last_x_assum $ qspecl_then [‘exp_size e’] assume_tac
+      \\ fs []
+      \\ pop_assum $ qspecl_then [‘e’] assume_tac
+      \\ fs []
+      \\ qabbrev_tac ‘ep = find_function e c’
+      \\ PairCases_on ‘ep’
+      \\ fs []
+      \\ first_x_assum dxrule
+      \\ rw []
+      \\ irule_at Any find_App
+      \\ first_assum $ irule_at Any >~[‘Var s’]
+      >- (irule_at Any find_Var
+          \\ qexists_tac ‘[]’
+          \\ fs []
+          \\ rw [FLOOKUP_UPDATE, dt_to_set_def])
+      \\ first_assum $ irule_at Any
+      \\ fs [])
+  >- (rw [find_function_def] (* Lam *)
+      \\ irule_at Any find_Bottom
+      \\ fs [])
+  >- (rw [find_function_def] (* Letrec *)
+      \\ irule_at Any find_Bottom
+      \\ fs [find_Bottom])
+QED
+
+
+Definition demand_analysis_def:
+  demand_analysis = SND o (λe. find_function e Nil)
+End
+
+Theorem demand_analysis_soundness:
+  ∀e. is_closed e ⇒ e ≈ demand_analysis e
+Proof
+  rw [demand_analysis_def]
+  \\ qabbrev_tac ‘p = find_function e Nil’
+  \\ PairCases_on ‘p’
+  \\ fs []
+  \\ irule find_soundness
+  \\ drule find_function_soundness_lemma
+  \\ rw []
+  \\ first_assum $ irule_at Any
+QED
+
+(*
   let foo = lam (a + 2) in
     lam x (foo x)
 -->
@@ -217,7 +1638,6 @@ End
     lam x (seq x (foo x))
 
   Letrec [(f,x)] rest
-
 *)
 
 val _ = export_theory();
